Simplify proofs for key expansion

src/crypto/aes/AES_helpers_i.fst
@@ -4,7 +4,6 @@ open Types_s
 open FStar.Seq
 open AES_s
 open FStar.Mul
-//open Calc
 
 // syntax for seq accesses, s.[index] and s.[index] <- value
 unfold
@@ -13,290 +12,108 @@ let op_String_Access (#a:Type) (s:seq a) (i:nat{ i < length s}) : Tot a = index 
 unfold
 let op_String_Assignment = Seq.upd
 
-let key_seq_type_helper (alg:algorithm) (key:seq nat32) : (key':seq nat32 { length key' == nk alg }) =
-  if length key = nk alg then key else create (nk alg) 0
+unfold let ( *^ ) = nat32_xor
+unfold let ( *^^ ) = quad32_xor
 
-let rec key_expansion_specific (alg:algorithm) (key:seq nat32 { length key == nk alg})
-                               (w:seq nat32) (i:nat{i < length w}) =
-    if 0 <= i && i < nk alg then
-      w.[i] == key.[i]
-    else
-      let temp = 
-        if i % (nk alg) = 0 then
-	  nat32_xor (sub_word (rot_word w.[i-1])) (aes_rcon ((i / (nk alg)) - 1))
-	else if nk alg > 6 && i % (nk alg) = 4 then
-	  sub_word w.[i-1]
-	else
-	  w.[i-1]
-      in 
-      w.[i] == nat32_xor w.[i - (nk alg)] temp
+let quad32_shl32 (q:quad32) : quad32 =
+  let Quad32 v0 v1 v2 v3 = q in
+  Quad32 0 v0 v1 v2
+
+assume val lemma_BitwiseXorCommutative (x y:nat32) : Lemma (x *^ y == y *^ x)
+assume val lemma_BitwiseXorWithZero (n:nat32) : Lemma (n *^ 0 == n)
+assume val lemma_BitwiseXorCancel (n:nat32) : Lemma (n *^ n == 0)
+assume val lemma_BitwiseXorAssociative (x y z:nat32) : Lemma (x *^ (y *^ z) == (x *^ y) *^ z)
+
+assume val xor_lemmas (_:unit) : Lemma
+  (ensures
+    (forall (x y:nat32).{:pattern (x *^ y)} x *^ y == y *^ x) /\
+    (forall (n:nat32).{:pattern (n *^ 0)} n *^ 0 == n) /\
+    (forall (n:nat32).{:pattern (n *^ n)} n *^ n == 0) /\
+    (forall (x y z:nat32).{:pattern (x *^ (y *^ z))} x *^ (y *^ z) == (x *^ y) *^ z)
+  )
+
+assume val lemma_RotWordSubWordCommutativity (x:nat32) : Lemma
+  (rot_word (sub_word x) == sub_word (rot_word x))
 
 
-let key_expansion_partial (alg:algorithm) (key:seq nat32 { length key == nk alg}) 
-                          (w:seq nat32) (end_index:nat{end_index <= length w}) = 
-  forall i .{:pattern (key_expansion_specific alg key w i)}
-    0 <= i /\ i < end_index ==> key_expansion_specific alg key w i
+// Redefine key expansion in terms of quad32 values rather than nat32 values,
+// then prove both definitions are equivalent.
 
-let lemma_selector255 (selector:nat8) (bits:bits_of_byte) : Lemma
-  (requires selector == 255 /\ bits == byte_to_twobits selector)
-  (ensures Bits_of_Byte?.lo bits == 3 /\ Bits_of_Byte?.mid_lo bits == 3 /\
-           Bits_of_Byte?.mid_hi bits == 3 /\ Bits_of_Byte?.hi bits == 3)
+let round_key_128_rcon (prev:quad32) (rcon:nat32) : quad32 =
+  let Quad32 v0 v1 v2 v3 = prev in
+  let w0 = v0 *^ (sub_word (rot_word v3) *^ rcon) in
+  let w1 = v1 *^ w0 in
+  let w2 = v2 *^ w1 in
+  let w3 = v3 *^ w2 in
+  Quad32 w0 w1 w2 w3
+
+let round_key_128 (prev:quad32) (round:nat) : quad32 =
+  round_key_128_rcon prev (aes_rcon (round - 1))
+
+let rec expand_key_128 (key:aes_key AES_128) (round:nat) : quad32 =
+  if round = 0 then Quad32 key.[0] key.[1] key.[2] key.[3]
+  else round_key_128 (expand_key_128 key (round - 1)) round
+
+#reset-options "--initial_fuel 4 --max_fuel 4 --max_ifuel 0 --z3rlimit 40"
+let lemma_expand_key_128_0 (key:aes_key AES_128) : Lemma
+  (equal key (expand_key AES_128 key 4))
+  = ()
+
+let lemma_expand_key_128_i (key:aes_key AES_128) (i:nat) : Lemma
+  (requires
+    0 < i /\ i < 11
+  )
+  (ensures (
+    let m = 4 * (i - 1) in
+    let n = 4 * i in
+    let v = expand_key AES_128 key n in
+    let w = expand_key AES_128 key (n + 4) in
+    let prev = Quad32 v.[m + 0] v.[m + 1] v.[m + 2] v.[m + 3] in
+    let Quad32 r0 r1 r2 r3 = round_key_128 prev i in
+    r0 == w.[n + 0] /\ r1 == w.[n + 1] /\ r2 == w.[n + 2] /\ r3 == w.[n + 3]
+  ))
+  = ()
+#reset-options
+
+// expand_key for large 'size' argument agrees with expand_key for smaller 'size' argument
+let rec lemma_expand_append (key:aes_key AES_128) (size1:nat) (size2:nat) : Lemma
+  (requires size1 <= size2 /\ size2 <= 44)
+  (ensures equal (expand_key AES_128 key size1) (slice (expand_key AES_128 key size2) 0 size1))
+  (decreases size2)
   =
-  ()
+  if size1 < size2 then lemma_expand_append key size1 (size2 - 1)
 
-assume val lemma_BitwiseXorCommutative (x y:nat32) : Lemma (nat32_xor x y == nat32_xor y x) 
-assume val lemma_BitwiseXorWithZero (n:nat32) : Lemma (nat32_xor n 0 == nat32_xor 0 n /\ nat32_xor 0 n == n)
-assume val lemma_double_xor_negates (x y z:nat32) : 
-  Lemma(
-    nat32_xor (nat32_xor x y) x == y /\
-    nat32_xor (nat32_xor x y) y == x /\
-    nat32_xor (nat32_xor x y) (nat32_xor x z) == nat32_xor y z)
-assume val lemma_BitwiseXorAssociative (x y z:nat32) : 
-  Lemma(nat32_xor x (nat32_xor y z) == nat32_xor (nat32_xor x y) z)
-assume val lemma_BitwiseXorAssociative2 (x y z p:nat32) :
-  Lemma(nat32_xor (nat32_xor x y) (nat32_xor z p) == nat32_xor (nat32_xor x z) (nat32_xor y p))
-assume val lemma_RotWordSubWordCommutativity (x:nat32) :
-  Lemma(rot_word (sub_word x) == sub_word (rot_word x))
+// quad32 key expansion is equivalent to nat32 key expansion
+let rec lemma_expand_key_128 (key:aes_key AES_128) (size:nat) : Lemma
+  (requires size <= 11)
+  (ensures (
+    let s = key_schedule_to_round_keys size (expand_key AES_128 key 44) in
+    (forall (i:nat).{:pattern (expand_key_128 key i)} i < size ==> expand_key_128 key i == s.[i])
+  ))
+  =
+  lemma_expand_append key (4 * size) 44;
+  if size = 0 then ()
+  else
+  (
+    let i = size - 1 in
+    lemma_expand_append key (4 * i) 44;
+    lemma_expand_key_128 key i;
+    if i = 0 then lemma_expand_key_128_0 key
+    else lemma_expand_key_128_i key i
+  )
 
-#reset-options "--z3rlimit 50"
+// Refine round_key_128 to a SIMD computation
+let simd_round_key_128 (prev:quad32) (rcon:nat32) : quad32 =
+  let r = rot_word (sub_word prev.hi) *^ rcon in
+  let q = prev in
+  let q = q *^^ quad32_shl32 q in
+  let q = q *^^ quad32_shl32 q in
+  let q = q *^^ quad32_shl32 q in
+  q *^^ Quad32 r r r r
 
-let lemma_KeyExpansionRoundHelperHelper (alg:algorithm) (key:seq nat32 { length key == nk alg})
-                                        (w_init w_final:seq nat32) (completed_bytes:int)
-					(xmm1_v9 : quad32) (important_value:nat32)
-					: Lemma
-  (requires 4 <= completed_bytes /\ completed_bytes <= 40 /\
-            alg == AES_128 /\
-            length w_init == 44 /\ length w_init == nb * (nr alg + 1) /\
-            key_expansion_partial alg key w_init completed_bytes /\
-            completed_bytes % 4 == 0 /\
-            length w_final == length w_init /\
-	    important_value == nat32_xor (rot_word (sub_word w_init.[completed_bytes-1])) (aes_rcon ((completed_bytes / nk(alg)) - 1)) /\
-	    xmm1_v9.lo == nat32_xor w_final.[completed_bytes-4] important_value /\
-	    xmm1_v9.mid_lo == nat32_xor(nat32_xor w_final.[completed_bytes-4] w_final.[completed_bytes-3]) important_value /\
-	    xmm1_v9.mid_hi == nat32_xor(nat32_xor w_final.[completed_bytes-2] (nat32_xor w_final.[completed_bytes-4] w_final.[completed_bytes-3])) important_value /\
-	    xmm1_v9.hi == nat32_xor(nat32_xor w_final.[completed_bytes-1] 
-					      (nat32_xor w_final.[completed_bytes-2]
-							 (nat32_xor w_final.[completed_bytes-4] w_final.[completed_bytes-3])))
-			            important_value /\
-	    (w_final == (let w = w_init.[completed_bytes]     <- xmm1_v9.lo in
-                         let w =      w.[completed_bytes + 1] <- xmm1_v9.mid_lo in
-                         let w =      w.[completed_bytes + 2] <- xmm1_v9.mid_hi in
-                         let w =      w.[completed_bytes + 3] <- xmm1_v9.hi in
-                         w)))
-  (ensures (key_expansion_partial alg key w_final (completed_bytes + 4)))
-=
-    lemma_RotWordSubWordCommutativity w_final.[completed_bytes-1];
-    //assert SubWord(RotWord(w_final.[completed_bytes-1])) == RotWord(SubWord(w_final.[completed_bytes-1]));
-
-    (*
-    calc {
-        w_final.[completed_bytes];
-        xmm1_v9.lo;
-        nat32_xor(w_final.[completed_bytes-4], important_value);
-        nat32_xor(w_final.[completed_bytes-4], nat32_xor(SubWord(RotWord(w_final.[completed_bytes-1])), AES_Rcon()[ (completed_bytes / Nk(alg))-1 ]));
-    }
-    *)
-    assert (w_final.[completed_bytes] == (nat32_xor w_final.[completed_bytes-4] (nat32_xor  (sub_word (rot_word w_final.[completed_bytes-1])) (aes_rcon ((completed_bytes / (nk alg))-1))))); 
-
-    let s:nat32 = xmm1_v9.mid_lo in
-    let t:nat32 = nat32_xor (nat32_xor w_final.[completed_bytes-4] w_final.[completed_bytes-3]) important_value in
-    let u:nat32 = nat32_xor (nat32_xor w_final.[completed_bytes-3] w_final.[completed_bytes-4]) important_value in
-    (*
-    calc (
-      s &= t &= u &| using (lemma_BitwiseXorCommutative w_final.[completed_bytes-4] w_final.[completed_bytes-3]; z3)
-      ); admit()
-     calc (
-           w_final.[completed_bytes+1]
-        &= s
-        //&= t
-       // &= u &| using (lemma_BitwiseXorCommutative w_final.[completed_bytes-4] w_final.[completed_bytes-3])
-
-       //&= nat32_xor w_final.[completed_bytes-3] (nat32_xor w_final.[completed_bytes-4] important_value) &| using (    lemma_BitwiseXorAssociative w_final.[completed_bytes-3] w_final.[completed_bytes-4] important_value)
-       //&= nat32_xor w_final.[completed_bytes-3] w_final.[completed_bytes]
-    );
-    admit()
-    *)
-
-    //calc {
-       // w_final.[completed_bytes+2];
-        //nat32_xor(nat32_xor(w_final.[completed_bytes-2], nat32_xor(w_final.[completed_bytes-4], w_final.[completed_bytes-3])), important_value);
-            lemma_BitwiseXorCommutative w_final.[completed_bytes-4] w_final.[completed_bytes-3]; 
-       // nat32_xor(nat32_xor(w_final.[completed_bytes-2], nat32_xor(w_final.[completed_bytes-3], w_final.[completed_bytes-4])), 32important_value);
-            lemma_BitwiseXorAssociative w_final.[completed_bytes-2] (nat32_xor w_final.[completed_bytes-3] w_final.[completed_bytes-4]) important_value;
-        //nat32_xor(w_final.[completed_bytes-2], nat32_xor(nat32_xor(w_final.[completed_bytes-3], w_final.[completed_bytes-4]), important_value));
-            lemma_BitwiseXorAssociative w_final.[completed_bytes-3] w_final.[completed_bytes-4] important_value;
-        //nat32_xor(w_final.[completed_bytes-2], nat32_xor(w_final.[completed_bytes-3], nat32_xor(w_final.[completed_bytes-4], important_value)));
-        //nat32_xor(w_final.[completed_bytes-2], nat32_xor(w_final.[completed_bytes-3], w_final.[completed_bytes]));
-        //nat32_xor(w_final.[completed_bytes-2], w_final.[completed_bytes+1]);
-    //}
-
-    //calc {
-    //    w_final.[completed_bytes+3];
-    //    nat32_xor(nat32_xor(w_final.[completed_bytes-1], nat32_xor(w_final.[completed_bytes-2], nat32_xor(w_final.[completed_bytes-4], w_final.[completed_bytes-3]))), important_value);
-    lemma_BitwiseXorCommutative w_final.[completed_bytes-4] w_final.[completed_bytes-3];
-   //     nat32_xor(nat32_xor(w_final.[completed_bytes-1], nat32_xor(w_final.[completed_bytes-2], nat32_xor(w_final.[completed_bytes-3], w_final.[completed_bytes-4]))), important_value);
-   lemma_BitwiseXorAssociative w_final.[completed_bytes-1] (nat32_xor w_final.[completed_bytes-2] (nat32_xor w_final.[completed_bytes-3] w_final.[completed_bytes-4])) important_value;
-    //    nat32_xor(w_final.[completed_bytes-1], nat32_xor(nat32_xor(w_final.[completed_bytes-2], nat32_xor(w_final.[completed_bytes-3], w_final.[completed_bytes-4])), important_value));
-   lemma_BitwiseXorCommutative w_final.[completed_bytes-4] w_final.[completed_bytes-3];
-    //    nat32_xor(w_final.[completed_bytes-1], nat32_xor(nat32_xor(w_final.[completed_bytes-2], nat32_xor(w_final.[completed_bytes-4], w_final.[completed_bytes-3])), important_value));
-    //    nat32_xor(w_final.[completed_bytes-1], w_final.[completed_bytes+2]);
-    //}
-   //let key_expansion_specific_restricted (i:int) = 0 <= i /\ i < completed_bytes ==> key_expansion_specific alg key w_final i in
-   (*
-   let lemma_KeyExpansionPredicateSpecific (i:int) : Lemma (ensures key_expansion_specific_restricted i) =
-     assert(0 <= i /\ i < completed_bytes ==> key_expansion_specific alg key w_init i)
-   in
-   Classical.forall_intro lemma_KeyExpansionPredicateSpecific;
-   assert(key_expansion_partial alg key w_final completed_bytes);
-   *)
-assume (key_expansion_partial alg key w_final completed_bytes);         //////////////////////////////////// TODO!
-
-(*
-    forall i | 0 <= i < completed_bytes
-        ensures KeyExpansionPredicateSpecific(key, alg, w, i);
-    {
-        assert KeyExpansionPredicateSpecific(key, alg, w_init, i);
-    }
-    assert KeyExpansionPredicatePartial(key, alg, w, completed_bytes);
-*)
-    //lemma_mod_auto(4);
-    (*
-    assert (completed_bytes+1)%4 == 1;
-    assert (completed_bytes+2)%4 == 2;
-    assert (completed_bytes+3)%4 == 3;
-    assert KeyExpansionPredicatePartial(key, alg, w, completed_bytes+4);
-  *)
-  admit()
-
-
-#reset-options "--z3rlimit 500"
-let lemma_KeyExpansionRoundHelper (alg:algorithm) (key:seq nat32 { length key == nk alg})
-                                  (w_init w_final:seq nat32) (completed_bytes:int)
-                                  (xmm1_v0 xmm2_v1 xmm2_v2 xmm3_v3 xmm1_v4 xmm3_v5 xmm1_v6 xmm3_v7 xmm1_v8 xmm1_v9 : quad32) 
-                                  : Lemma
-  (requires 4 <= completed_bytes /\ completed_bytes <= 40 /\
-            alg == AES_128 /\
-            length w_init == 44 /\ length w_init == nb * (nr alg + 1) /\
-            key_expansion_partial alg key w_init completed_bytes /\
-            completed_bytes % 4 == 0 /\
-            length w_final == length w_init /\
-            xmm1_v0 == Quad32 w_final.[completed_bytes-4] 
-                              w_final.[completed_bytes-3] 
-                              w_final.[completed_bytes-2]
-                              w_final.[completed_bytes-1] /\
-
-            (let rcon = aes_rcon((completed_bytes / nk(alg)) - 1) in
-
-            xmm2_v1 == Quad32 (sub_word xmm1_v0.mid_lo) (nat32_xor (rot_word (sub_word xmm1_v0.mid_lo)) rcon) (sub_word xmm1_v0.hi) (nat32_xor (rot_word (sub_word xmm1_v0.hi)) rcon)) /\
-
-            (let bits = byte_to_twobits 255 in
-            xmm2_v2 == Quad32 (select_word xmm2_v1 (Bits_of_Byte?.lo bits)) 
-                              (select_word xmm2_v1 (Bits_of_Byte?.mid_lo bits))
-                              (select_word xmm2_v1 (Bits_of_Byte?.mid_hi bits))
-                              (select_word xmm2_v1 (Bits_of_Byte?.hi bits))) /\
-            xmm3_v3 == Quad32 0 xmm1_v0.lo xmm1_v0.mid_lo xmm1_v0.mid_hi /\
-            xmm1_v4 == quad32_xor xmm1_v0 xmm3_v3 /\
-            xmm3_v5 == Quad32 0 xmm1_v4.lo xmm1_v4.mid_lo xmm1_v4.mid_hi /\
-            xmm1_v6 == quad32_xor xmm1_v4 xmm3_v5 /\
-            xmm3_v7 == Quad32 0 xmm1_v6.lo xmm1_v6.mid_lo xmm1_v6.mid_hi /\
-            xmm1_v8 == quad32_xor xmm1_v6 xmm3_v7 /\
-            xmm1_v9 == quad32_xor xmm1_v8 xmm2_v2 /\
-            
-            (w_final == (let w = w_init.[completed_bytes]     <- xmm1_v9.lo in
-                         let w =      w.[completed_bytes + 1] <- xmm1_v9.mid_lo in
-                         let w =      w.[completed_bytes + 2] <- xmm1_v9.mid_hi in
-                         let w =      w.[completed_bytes + 3] <- xmm1_v9.hi in
-                         w)))
-  (ensures (key_expansion_partial alg key w_final (completed_bytes + 4)))
-  = 
-  let transformed_w_init_val:nat32 = rot_word (sub_word (index w_init (completed_bytes - 1))) in
-  let rcon_index:int = (completed_bytes / (nk alg)) - 1 in 
-  let aes_rcon_val:nat32 = aes_rcon rcon_index in
-  let important_value = nat32_xor transformed_w_init_val aes_rcon_val in
-  let bits = byte_to_twobits 255 in
-  lemma_selector255 255 bits;
-  assert (xmm2_v2.mid_lo == important_value); 
-  assert (xmm2_v2.mid_hi == important_value); 
-  lemma_BitwiseXorWithZero w_final.[completed_bytes-4];
-  lemma_BitwiseXorCommutative w_final.[completed_bytes-3] w_final.[completed_bytes-4];
-  lemma_double_xor_negates w_final.[completed_bytes-4] w_final.[completed_bytes-3] 0;
-  lemma_BitwiseXorCommutative w_final.[completed_bytes-2] w_final.[completed_bytes-3];
-  lemma_double_xor_negates w_final.[completed_bytes-3] w_final.[completed_bytes-2] w_final.[completed_bytes-4];
-
-  // Calc 1
-  // nat32_xor (nat32_xor w_final.[completed_bytes-1] w_final.[completed_bytes-2]) (nat32_xor w_final.[completed_bytes-2] w_final.[completed_bytes-3]
-  lemma_BitwiseXorCommutative w_final.[completed_bytes-1] w_final.[completed_bytes-2];
-  // nat32_xor (nat32_xor w_final.[completed_bytes-2] w_final.[completed_bytes-1]) (nat32_xor w_final.[completed_bytes-2] w_final.[completed_bytes-3]
-  lemma_double_xor_negates w_final.[completed_bytes-2] w_final.[completed_bytes-1] w_final.[completed_bytes-3];
-  // nat32_xor w_final.[completed_bytes-1], w_final.[completed_bytes-3]
-  lemma_BitwiseXorCommutative w_final.[completed_bytes-1] w_final.[completed_bytes-3];
-  //nat32_xor w_final.[completed_bytes-3], w_final.[completed_bytes-1]
-
-  // Calc 2
-  // nat32_xor (nat32_xor w_final.[completed_bytes-2] w_final.[completed_bytes-4]), w_final.[completed_bytes-3];
-  lemma_BitwiseXorAssociative w_final.[completed_bytes-2] w_final.[completed_bytes-4] w_final.[completed_bytes-3];
-  // nat32_xor w_final.[completed_bytes-2] (nat32_xor w_final.[completed_bytes-4], w_final.[completed_bytes-3]);
-    
-  // Calc 3
-  
-  // (nat32_xor (nat32_xor w_final.[completed_bytes-3], w_final.[completed_bytes-1]), (nat32_xor w_final.[completed_bytes-2], w_final.[completed_bytes-4]));
-  lemma_BitwiseXorCommutative w_final.[completed_bytes-3] w_final.[completed_bytes-1];
-  // (nat32_xor (nat32_xor w_final.[completed_bytes-1], w_final.[completed_bytes-3]), (nat32_xor w_final.[completed_bytes-2], w_final.[completed_bytes-4]));
-  lemma_BitwiseXorAssociative2 w_final.[completed_bytes-1] w_final.[completed_bytes-3] w_final.[completed_bytes-2] w_final.[completed_bytes-4];
-  //(nat32_xor (nat32_xor w_final.[completed_bytes-1], w_final.[completed_bytes-2]), (nat32_xor w_final.[completed_bytes-3], w_final.[completed_bytes-4]));
-  //(nat32_xor (nat32_xor w_final.[completed_bytes-1], w_final.[completed_bytes-2]), (nat32_xor w_final.[completed_bytes-4], w_final.[completed_bytes-3]));
-  lemma_BitwiseXorAssociative w_final.[completed_bytes-1] w_final.[completed_bytes-2] (nat32_xor w_final.[completed_bytes-4] w_final.[completed_bytes-3]);
-  //(nat32_xor w_final.[completed_bytes-1], (nat32_xor w_final.[completed_bytes-2], (nat32_xor w_final.[completed_bytes-4], w_final.[completed_bytes-3])));
-
-  lemma_KeyExpansionRoundHelperHelper alg key w_init w_final completed_bytes xmm1_v9 important_value;
-  ()
-
-(*
-{
-    var important_value := BitwiseXor(RotWord(SubWord(w_init[completedBytes-1])), AES_Rcon()[ (completedBytes / Nk(alg))-1 ]);
-    var bits := byte_to_bits(255);
-    lemma_Selector255(255, bits);
-    calc {
-        xmm2_v2.mid_lo;
-        select_word(xmm2_v1, bits.mid_lo);
-        xmm2_v1.hi;
-        important_value;
-    }
-    calc {
-        xmm2_v2.mid_hi;
-        select_word(xmm2_v1, bits.mid_hi);
-        xmm2_v1.hi;
-        important_value;
-    }
-    lemma_BitwiseXorWithZero(w[completedBytes-4]);
-    lemma_BitwiseXorCommutative(w[completedBytes-3], w[completedBytes-4]);
-    lemma_double_xor_negates(w[completedBytes-4], w[completedBytes-3], 0);
-    lemma_BitwiseXorCommutative(w[completedBytes-2], w[completedBytes-3]);
-    lemma_double_xor_negates(w[completedBytes-3], w[completedBytes-2], w[completedBytes-4]);
-    calc {
-        BitwiseXor(BitwiseXor(w[completedBytes-1], w[completedBytes-2]), BitwiseXor(w[completedBytes-2], w[completedBytes-3]));
-            { lemma_BitwiseXorCommutative(w[completedBytes-1], w[completedBytes-2]); }
-        BitwiseXor(BitwiseXor(w[completedBytes-2], w[completedBytes-1]), BitwiseXor(w[completedBytes-2], w[completedBytes-3]));
-            { lemma_double_xor_negates(w[completedBytes-2], w[completedBytes-1], w[completedBytes-3]); }
-        BitwiseXor(w[completedBytes-1], w[completedBytes-3]);
-            { lemma_BitwiseXorCommutative(w[completedBytes-1], w[completedBytes-3]); }
-        BitwiseXor(w[completedBytes-3], w[completedBytes-1]);
-    }
-    calc {
-        BitwiseXor(BitwiseXor(w[completedBytes-2], w[completedBytes-4]), w[completedBytes-3]);
-            { lemma_BitwiseXorAssociative(w[completedBytes-2], w[completedBytes-4], w[completedBytes-3]); }
-        BitwiseXor(w[completedBytes-2], BitwiseXor(w[completedBytes-4], w[completedBytes-3]));
-    }
-    calc {
-        BitwiseXor(BitwiseXor(w[completedBytes-3], w[completedBytes-1]), BitwiseXor(w[completedBytes-2], w[completedBytes-4]));
-            { lemma_BitwiseXorCommutative(w[completedBytes-3], w[completedBytes-1]); }
-        BitwiseXor(BitwiseXor(w[completedBytes-1], w[completedBytes-3]), BitwiseXor(w[completedBytes-2], w[completedBytes-4]));
-            { lemma_BitwiseXorAssociative2(w[completedBytes-1], w[completedBytes-3], w[completedBytes-2], w[completedBytes-4]); }
-        BitwiseXor(BitwiseXor(w[completedBytes-1], w[completedBytes-2]), BitwiseXor(w[completedBytes-3], w[completedBytes-4]));
-        BitwiseXor(BitwiseXor(w[completedBytes-1], w[completedBytes-2]), BitwiseXor(w[completedBytes-4], w[completedBytes-3]));
-            { lemma_BitwiseXorAssociative(w[completedBytes-1], w[completedBytes-2], BitwiseXor(w[completedBytes-4], w[completedBytes-3])); }
-        BitwiseXor(w[completedBytes-1], BitwiseXor(w[completedBytes-2], BitwiseXor(w[completedBytes-4], w[completedBytes-3])));
-    }
-    lemma_KeyExpansionRoundHelperHelper(key, alg, w_init, completedBytes, xmm1_v9, important_value, w);
-}
-*)
+// SIMD version of round_key_128 is equivalent to scalar round_key_128
+let lemma_simd_round_key (prev:quad32) (rcon:nat32) : Lemma
+  (simd_round_key_128 prev rcon == round_key_128_rcon prev rcon)
+  =
+  lemma_RotWordSubWordCommutativity prev.hi;
+  xor_lemmas ()
